OpenLocalTableau.paths_nonempty
This adjust the the BuildTree.loc constructor in two ways:
- restrict the choice of prover to open local tableau that
  have at least one end node.
- add someLT saying "there is at least one open local tableau"
  analogous to the recently added someR for PDL rules.

Together this should be enough information based on the fact that prover
cannot win, by assumption when running buildTree to make a BuildTree.

Pdl/BuildTree.lean
@@ -60,6 +60,23 @@ lemma FreeRepeat_nil_impossible : FreeRepeat [] X → False := by
   rintro ⟨n, n_h⟩
   grind
 
+/-- An open local tableau has at least one end node. -/
+def OpenLocalTableau (X : Sequent) : Type := {lt : LocalTableau X // endNodesOf lt ≠ []}
+deriving DecidableEq
+
+def OpenLocalTableau.all (X : Sequent) : List (OpenLocalTableau X) :=
+  ((LocalTableau.all X).filter (endNodesOf · ≠ [])).attach.map (fun ⟨lt,h⟩ => ⟨lt, by simp_all⟩)
+
+lemma OpenLocalTableau.all_spec {X : Sequent} {ltX : OpenLocalTableau X} :
+    ltX ∈ OpenLocalTableau.all X := by
+  rcases ltX with ⟨lt, lt_has_ends⟩
+  unfold all
+  simp_all only [ne_eq, List.mem_map, List.mem_attach, true_and, Subtype.exists, decide_not,
+    List.mem_filter, Bool.not_eq_eq_eq_not, Bool.not_true, decide_eq_false_iff_not]
+  use lt
+  have := lt.all_spec
+  grind
+
 mutual
 /-- Winning Strategy Tree for Builder.
 At each step, we consider
@@ -73,9 +90,9 @@ Instead of the .lpr constructor here we have .fpr because we only make a `RuleTr
 wins and thus we can never reach an lpr where Prover would win, but do allow free repeats.
 As in `Tableau` note that the history is stored in reverse. -/
 inductive BuildTree : History → Sequent → Type
-  /-- Prover chooses local tab, we pick one end node. -/
-  | loc {H X} (nbas : ¬ X.basic)
-            (next : (lt : LocalTableau X) → BuildChoice H X (endNodesOf lt))
+  /-- Prover chooses local tab, we pick an end node (which must exist as otherwise prover wins). -/
+  | loc {H X} (nbas : ¬ X.basic) (someLT : OpenLocalTableau.all X ≠ [])
+            (next : (lt : OpenLocalTableau X) → BuildChoice H X (endNodesOf lt.1))
             : BuildTree H X
   /-- Prover chooses PDL rule, never branches, so continue with unique child. -/
   | pdl {H X} (bas : X.basic) (someR : PdlRule.all X ≠ [])
@@ -98,7 +115,7 @@ end
 mutual
 /-- Manual replacement for `sizeOf (bt : BuildTree)` so we also count the `next` parts. -/
 def BuildTree.size : BuildTree H X → Nat
-  | .loc _ next => 1 + ((LocalTableau.all X).map (fun lt => (next lt).size)).sum
+  | .loc _ _ next => 1 + ((OpenLocalTableau.all X).map (fun lt => (next lt).size)).sum
   | .pdl _ _ next => 1 + ((PdlRule.all X).map (fun ⟨Y,r⟩ => (next Y r).size)).sum
   | .freeRepeat _ => 1
   | .openLeaf _ _ => 1
@@ -108,12 +125,13 @@ def BuildChoice.size : BuildChoice H X YS → Nat
 end
 
 lemma BuildTree.size_lt_loc (H : History) (X : Sequent) (nbas : ¬X.basic)
-    (next : (lt : LocalTableau X) → BuildChoice H X (endNodesOf lt)) (ltX : LocalTableau X) :
-    (next ltX).6.size < (BuildTree.loc nbas next).size := by
+    (next : (lt : OpenLocalTableau X) → BuildChoice H X (endNodesOf lt.1))
+    (ltX : OpenLocalTableau X) someLT :
+    (next ltX).6.size < (BuildTree.loc nbas someLT next).size := by
   simp [BuildTree.size]
-  have : (next ltX).6.size ∈ ((LocalTableau.all X).map (fun lt => (next lt).6.size)) := by
+  have : (next ltX).6.size ∈ ((OpenLocalTableau.all X).map (fun lt => (next lt).6.size)) := by
     simp only [List.mem_map]
-    use ltX, LocalTableau.all_spec
+    use ltX, OpenLocalTableau.all_spec
   have := List.le_sum_of_mem this
   have : ∀ lt, (next lt).size = (next lt).6.size := fun lt => by
     cases next lt; simp [BuildChoice.size]
@@ -204,14 +222,24 @@ def buildTree (s : Strategy tableauGame Builder) {H X p} (h : winning s ⟨H, X,
       have stillWin : ∀ newP, ∀ _ : Move ⟨_,_,Sum.inl (.nbas nrep nbas)⟩ newP, winning s newP :=
         fun newPos mov =>
           @winning_of_whatever_other_move _ _ s _ (by simp) h ⟨newPos, mem_theMoves_of_move ⟨mov⟩⟩
-      .loc nbas <| fun ltX => by
-        have ne : (tableauGame.moves ⟨H, ⟨X, Sum.inr (BuilderPos.ltab nrep nbas ltX)⟩⟩).Nonempty :=
+      have someLT : OpenLocalTableau.all X ≠ [] := by
+        -- We show that there is no lt without end nodes because prover could use it to win.
+        rcases List.exists_mem_of_ne_nil _ (LocalTableau.all_nonempty X) with ⟨lt, lt_in⟩
+        apply List.ne_nil_of_mem (@OpenLocalTableau.all_spec X ⟨lt, ?_⟩)
+        intro lt_no_ends
+        have := stillWin ⟨H, ⟨X, Sum.inr (.ltab nrep nbas lt)⟩⟩ Move.prLocTab
+        have has_moves := winning_has_moves (by simp) this
+        simp only [tableauGame, Game.moves, theMoves, List.toFinset_nonempty_iff, ne_eq,
+          List.map_eq_nil_iff] at has_moves
+        exact has_moves lt_no_ends
+      .loc nbas someLT <| fun ltX => by
+        have ne : (tableauGame.moves ⟨H, ⟨X, Sum.inr (.ltab nrep nbas ltX.1)⟩⟩).Nonempty :=
           winning_has_moves (by simp) <|
-            stillWin ⟨H, ⟨X, Sum.inr (BuilderPos.ltab nrep nbas ltX)⟩⟩ Move.prLocTab
+            stillWin ⟨H, ⟨X, Sum.inr (.ltab nrep nbas ltX.1)⟩⟩ Move.prLocTab
         -- IDEA: use strategy `s` to choose move `mY` that picks the `Y ∈ endNodeOf ltX`:
         -- We want to define mY and then do rcases, but keep the information how it was defined.
-        let mY_raw := s ⟨H, X, Sum.inr (.ltab nrep nbas ltX)⟩ (by simp) ne
-        have mY_def : mY_raw.1 = s ⟨H, X, Sum.inr (.ltab nrep nbas ltX)⟩ (by simp) ne := rfl
+        let mY_raw := s ⟨H, X, Sum.inr (.ltab nrep nbas ltX.1)⟩ (by simp) ne
+        have mY_def : mY_raw.1 = s ⟨H, X, Sum.inr (.ltab nrep nbas ltX.1)⟩ (by simp) ne := rfl
         rcases mY_raw with ⟨mY, mY_prop⟩
         simp at mY_def
         -- We continue the BuildTree with the chosen `Y`:
@@ -226,12 +254,12 @@ def buildTree (s : Strategy tableauGame Builder) {H X p} (h : winning s ⟨H, X,
           simp
           exact Y'_in
         · -- now still need to make a `Move` so we can recursively call `buildTree`.
-          have Mov : Move ⟨H, X, Sum.inr (.ltab nrep nbas ltX)⟩ mY := by
+          have Mov : Move ⟨H, X, Sum.inr (.ltab nrep nbas ltX.1)⟩ mY := by
             simp only [Game.Pos.moves, tableauGame, theMoves, List.mem_toFinset] at mY_prop
             simp [List.mem_map] at mY_prop
             let oY := List.find? -- No more choice thanks to this!
               (fun Y => @decide (⟨_, ⟨_, posOf (X :: H) Y⟩⟩ = mY) (instDecidableEqPos _ _))
-              (endNodesOf ltX)
+              (endNodesOf ltX.1)
             cases oY_def : oY
             · exfalso
               have := List.find?_eq_none.mp oY_def
@@ -241,7 +269,7 @@ def buildTree (s : Strategy tableauGame Builder) {H X p} (h : winning s ⟨H, X,
               have def_mY := List.find?_some oY_def
               simp only [decide_eq_true_eq] at def_mY
               have Y_in := List.mem_of_find?_eq_some oY_def
-              have := @Move.buEnd X ltX Y H nrep nbas Y_in
+              have := @Move.buEnd X ltX.1 Y H nrep nbas Y_in
               rw [← def_mY]
               exact this
           rcases mY with ⟨H', Y, newP⟩ -- Happy because this does not lose mY_def.
@@ -258,7 +286,7 @@ def buildTree (s : Strategy tableauGame Builder) {H X p} (h : winning s ⟨H, X,
                 unfold WellFoundedRelation.rel Game.wf tableauGame
                 simp
                 apply @Relation.TransGen.trans _ _ _
-                  ⟨H, ⟨X, Sum.inr (BuilderPos.ltab nrep nbas ltX)⟩⟩
+                  ⟨H, ⟨X, Sum.inr (BuilderPos.ltab nrep nbas ltX.1)⟩⟩
                 · exact Relation.TransGen.single ⟨Mov⟩
                 · rw [p_def]; exact Relation.TransGen.single ⟨Move.prLocTab⟩
             refine H'_def ▸ @buildTree s H' Y myP ?_
@@ -267,7 +295,7 @@ def buildTree (s : Strategy tableauGame Builder) {H X p} (h : winning s ⟨H, X,
             -- Note that *two* moves have happened now, one by prover and one by Builder using `s`.
             -- Remains to show that `s` still wins.
             apply winning_of_winning_move
-            exact stillWin ⟨_, X, Sum.inr (BuilderPos.ltab nrep nbas ltX)⟩ Move.prLocTab
+            exact stillWin ⟨_, X, Sum.inr (BuilderPos.ltab nrep nbas ltX.1)⟩ Move.prLocTab
           | .inr mY_BP =>
               exfalso -- fingers crossed ;-)
               subst H'_def
@@ -282,7 +310,7 @@ def buildTree (s : Strategy tableauGame Builder) {H X p} (h : winning s ⟨H, X,
                   simp [winning] at this
                 rw [mY_def]
                 apply @winning_of_winning_move _ _ s
-                exact stillWin ⟨_, X, Sum.inr (BuilderPos.ltab nrep nbas ltX)⟩ Move.prLocTab
+                exact stillWin ⟨_, X, Sum.inr (BuilderPos.ltab nrep nbas ltX.1)⟩ Move.prLocTab
               case ltab => -- impossible
                 clear mY_def mY_prop newP
                 have := mem_theMoves_of_move (⟨Mov⟩)
@@ -307,7 +335,7 @@ this could be called a "rollout", but note that it stays within the given Builde
 and it is not tracking all intermediate game positions. -/
 inductive Match : ∀ {H : History} {X : Sequent}, BuildTree H X → Type
   | nil {bt} : Match bt
-  | loc {nbas next lt} : Match (next lt).6 → Match (BuildTree.loc nbas next)
+  | loc {nbas someLT next lt} : Match (next lt).6 → Match (BuildTree.loc nbas someLT next)
   | pdl {bas someR next Y r} : Match (next Y r) → Match (BuildTree.pdl bas someR next)
 deriving DecidableEq
 
@@ -329,9 +357,9 @@ def Match.endSeq {bt : BuildTree H X} (m : Match bt) : Sequent := m.btAt.2.1
 
 /- All possible Matches in a given BuildTree. -/
 def Match.all {H X} : (bt : BuildTree H X) → List (Match bt)
-  | .loc nbas next =>
+  | .loc nbas someLT next =>
       Match.nil ::
-      (LocalTableau.all X >>= fun ltX => return Match.loc (← Match.all (next ltX).6))
+      (OpenLocalTableau.all X >>= fun ltX => return Match.loc (← Match.all (next ltX).6))
   | .pdl bas someRule next =>
       Match.nil ::
       (PdlRule.all X >>= fun ⟨Y,r⟩ => return Match.pdl (← (Match.all (next Y r))))
@@ -346,12 +374,12 @@ decreasing_by
 theorem Match.all_spec {H X} {bt : BuildTree H X} {m} :
     m ∈ Match.all bt := match m with
   | nil => by cases bt <;> grind [Match.all]
-  | @loc _ _ bas next lt tail => by
+  | @loc _ _ bas someLT next lt tail => by
     have IH:= @Match.all_spec _ _ _ tail
     rw[Match.all]
     simp
     refine ⟨lt,?_ ⟩
-    refine ⟨ LocalTableau.all_spec ,tail,IH,?_⟩
+    refine ⟨ OpenLocalTableau.all_spec ,tail,IH,?_⟩
     simp
   | @pdl _ _ bas someR next Y r tail => by
     have IH := @Match.all_spec _ _ _ tail
@@ -414,8 +442,8 @@ def Match.rewind {H X} {bt : BuildTree H X} : (m : Match bt) → (k : Fin (m.len
 @[simp]
 lemma Match.rewind_zero {H X} {bt : BuildTree H X} (m : Match bt) : m.rewind 0 = m := by
   induction m <;> simp only [rewind]
-  case loc H X nbas next lt tail IH => -- idea from PathIn.rewind_zero
-    have : 0 ≠ Fin.last (@loc H X nbas next lt tail).length := by
+  case loc H X nbas someLT next lt tail IH => -- idea from PathIn.rewind_zero
+    have : 0 ≠ Fin.last (@loc H X nbas someLT next lt tail).length := by
       simp_all [Fin.last]
     rw [← Fin.exists_castSucc_eq] at this
     rcases this with ⟨k,kdef⟩
@@ -460,7 +488,7 @@ lemma Match.btAt_newHist_length_eq_length_plus_oldHist {H X} {bt : BuildTree H X
     m.btAt.1.length = m.length + H.length :=
   match m with
   | nil => by simp [btAt]
-  | @loc _ _ _ next lt tail => by
+  | @loc _ _ _ _ next lt tail => by
     have IH := Match.btAt_newHist_length_eq_length_plus_oldHist tail
     unfold btAt
     rw [IH]
@@ -526,6 +554,7 @@ lemma Sequent.mem_bothSides_iff (φ : Formula) (X : Sequent) :
 
 This may be useful for the pre-states used in the completeness proof. -/
 
+-- TODO golf/shorten this
 /-- LocalRuleApp preserves saturatedness backwards. -/
 lemma LocalRuleApp.preserve_saturated_up (lra : LocalRuleApp) :
     ∀ Y ∈ lra.C, ∀ (rest : List Sequent) ,
@@ -596,7 +625,8 @@ lemma LocalRuleApp.preserve_saturated_up (lra : LocalRuleApp) :
         exact ⟨Fδ, hD, by simpa using fun f hf => lift_rest _ (by simpa using hF f hf)⟩
       · rcases (hexpand φ ψ α).2.2.2.2 rfl with ⟨Fδ, hD, hF⟩
         simp only [List.all_eq_true, decide_eq_true_eq] at hF
-        exact ⟨Fδ, hD, by simpa using fun f hf => lift_rest _ (child_in_rest _ (by simpa using hF f hf))⟩
+        exact ⟨ Fδ, hD
+              , by simpa using fun f hf => lift_rest _ (child_in_rest _ (by simpa using hF f hf))⟩
     · rcases hdia hrest with ⟨Fδ, hD, hF⟩
       simp only [List.all_eq_true, decide_eq_true_eq] at hF
       exact ⟨Fδ, hD, by simpa using fun f hf => lift_rest _ (by simpa using hF f hf)⟩
@@ -610,15 +640,6 @@ termination_by
 decreasing_by
   subst_eqs
   apply localRuleApp.decreases_DM lra Y h
-
-lemma LocalTableau.paths_nonempty {X} (lt : LocalTableau X) :
-    lt.paths ≠ [] := by
-  cases lt <;> simp [paths]
-  case byLocalRule lra next def_X =>
-    subst def_X
-    -- WORRY: what if the lra has no results because it's a "contradiction/closing" rule?
-    -- maybe we need the additional assumption here that X is consistent?
-    sorry
 
 lemma LocalTableau.paths_mem_nonempty {X} (lt : LocalTableau X) :
     ∀ L ∈ lt.paths, L ≠ [] := by
@@ -686,6 +707,14 @@ lemma LocalTableau.pathsLast_eq_endNodes {X} {lt : LocalTableau X} :
     ext
     simp [paths]
     grind
+
+/-- Any open local tableau has at least one path (from root to some end node).
+Does not hold for `LocalTableau` which might end with "contradiction/closing" rule applications. -/
+lemma OpenLocalTableau.paths_nonempty {X} (lt : OpenLocalTableau X) :
+    lt.1.paths ≠ [] := by
+  rcases lt with ⟨lt, lt_has_ends⟩
+  have := @LocalTableau.pathsLast_eq_endNodes X lt
+  grind
 
 lemma LocalTableau.paths_last_basic {X} {lt : LocalTableau X} :
     ∀ L, (h : L ∈ lt.paths) → (L.getLast (LocalTableau.paths_mem_nonempty lt L h)).basic := by
@@ -765,34 +794,35 @@ decreasing_by
   subst_eqs
   exact localRuleApp.decreases_DM _ _ Y_in
 
-/-! ## Collecting Sequents for Pre-states NEW APPROACH - directly from BuildTree ??
+/-! ## Collecting Sequents for Pre-states
 
 As possible worlds for the model graph we want to define *maximal* paths inside the build tree
-that do not contain (M), (L+) or (L-) steps. -/
+that do not contain (M), (L+) or (L-) steps.
+
+We collect the sequents along such paths directly by induction on the `BuildTree`. -/
 
 /-- Collect pre-states in the whole BuildTree.
 The local pre-states come from paths in a local tableau,
 and PDL pre-states each consist of just a single node. -/
 def BuildTree.collect {H X} : (bt : BuildTree H X) → List (List Sequent)
-  | .loc _ next => (LocalTableau.all X).flatMap fun lt => lt.paths ++ (next lt).6.collect
+  | .loc _ _ next => (OpenLocalTableau.all X).flatMap fun lt => lt.1.paths ++ (next lt).6.collect
   | .pdl _ _ next => [ [X] ] ++ (PdlRule.all X).flatMap fun ⟨Y,r⟩ => (next Y r).collect
   | .freeRepeat _ => [ ] -- Not generating a pre-state here, go to companion instead !! ?? !!
   | .openLeaf _ _ => [ [X] ]
 termination_by
   bt => bt.size -- size of remaining BuildTree should go down
 decreasing_by
-  · exact size_lt_loc H X _ next lt
+  · exact size_lt_loc H X _ next lt _
   · exact size_lt_pdl H X _ _ next Y r
 
 lemma BuildTree.collect_nonempty (bt : BuildTree [] X) :
     bt.collect ≠ [] := by
   cases bt
-  case loc nbas next =>
+  case loc nbas someLT next =>
     simp only [collect, ne_eq, List.flatMap_eq_nil_iff, List.append_eq_nil_iff, not_forall, not_and]
-    have := LocalTableau.all_nonempty X
-    rcases List.exists_mem_of_ne_nil _ this with ⟨lt, lt_in⟩
+    rcases List.exists_mem_of_ne_nil _ someLT with ⟨lt, lt_in⟩
     use lt, lt_in
-    have := LocalTableau.paths_nonempty lt
+    have := OpenLocalTableau.paths_nonempty lt -- new :-)
     tauto
   all_goals
     simp [collect]
@@ -802,15 +832,13 @@ lemma BuildTree.collect_nonempty (bt : BuildTree [] X) :
 lemma BuildTree.collect_contains_root (bt : BuildTree [] X) :
     ∃ π ∈ bt.collect, X ∈ π := by
   cases bt <;> simp [collect]
-  case loc nbas next =>
-    let lts := LocalTableau.all X
-    have lts_ne : lts ≠ [] := LocalTableau.all_nonempty X
-    rcases lts.exists_mem_of_ne_nil lts_ne with ⟨lt, lt_in⟩
-    let πs := lt.paths
-    have πs_ne : πs ≠ [] := LocalTableau.paths_nonempty lt
+  case loc nbas someLT next =>
+    rcases List.exists_mem_of_ne_nil _ someLT with ⟨lt, lt_in⟩
+    let πs := lt.1.paths
+    have πs_ne : πs ≠ [] := OpenLocalTableau.paths_nonempty lt
     rcases πs.exists_mem_of_ne_nil πs_ne with ⟨π, π_in⟩
     refine ⟨π, ⟨lt, lt.all_spec, .inl π_in⟩, ?_⟩
-    have := @LocalTableau.pathsHead_eq_self X lt π
+    have := @LocalTableau.pathsHead_eq_self X lt.1 π
     grind
   case freeRepeat h =>
     exact FreeRepeat_nil_impossible h
@@ -825,11 +853,11 @@ lemma PreState.nonempty {X} {bt : BuildTree H X} {π : PreState bt} : π.val ≠
   unfold BuildTree.collect at L_in
   simp_all
   cases bt
-  case loc nbas next L_in' =>
+  case loc nbas someLT next L_in' =>
     simp_all
     rcases L_in with ⟨lt, lt_in, L_in⟩
     rcases L_in with L_in|L_in
-    · exact LocalTableau.paths_mem_nonempty lt L L_in
+    · exact LocalTableau.paths_mem_nonempty lt.1 L L_in
     · have IH := @PreState.nonempty _ _ (next lt).6 ⟨L, L_in⟩
       exact IH
   case pdl bas next L_in' =>
